


infixl 15 _-_
_-_ : ℕ → ℕ → ℕ
m - Z = m
Z - S n = Z  
S m - S n = (m - n)


_ : 2 - 3 ≡ 0
_ = ↯

_ : 3 - 1 ≡ 2
_ = ↯


infixl 16 _%_
_%_ : ℕ → ℕ → ℕ
Z % n = Z
(S m) % n with _⋚?_ (n - 1) (m % n)
(S m) % n | [<] = S(m % n)
(S m) % n | [≡] = Z
(S m) % n | [>] = S(m % n)

_ : 2 % 3 ≡ 2
_ = ↯

_ : 5 % 3 ≡ 2
_ = ↯

_ : 0 % 0 ≡ 0
_ = ↯

_ : 2 % 2 ≡ 0
_ = ↯

_ : 10 % 2 ≡ 0
_ = ↯


infixl 16 _/_
_/_ : ℕ → ℕ → ℕ
Z / n = Z
S m / n with _⋚?_ (m % n) (n - 1)
(S m / n) | [<] = m / n
(S m / n) | [≡] = S(m / n)
(S m / n) | [>] = m / n


_ : 2 / 3 ≡ 0
_ = ↯

_ : 5 / 2 ≡ 2
_ = ↯

_ : 0 / 0 ≡ 0
_ = ↯

_ : 2 / 2 ≡ 1
_ = ↯

_ : 10 / 2 ≡ 5
_ = ↯
